formal/nightstream-lean/CheckCli.lean
@@ -4,6 +4,11 @@ import Nightstream.Rv64IM.Checks
 import Nightstream.Rv64IM.AcceptedArtifactChecks
 import Nightstream.Rv64IM.AcceptedArtifactCompleteness
 import Nightstream.Rv64IM.AcceptedArtifactConstructorAudit
+import Nightstream.Rv64IM.AcceptedArtifactKernelDesignBridgeClosure
+import Nightstream.Rv64IM.AcceptedArtifactRootExecutionClosure
+import Nightstream.Rv64IM.AcceptedArtifactRootExecutionSemanticsClosure
+import Nightstream.Rv64IM.AcceptedArtifactBackendRefinement
+import Nightstream.Rv64IM.ProofCompleteAudit
 
 def main : IO UInt32 := do
   IO.println s!"chip8_transcript_vector_checks={Nightstream.Chip8.transcriptVectorChecks}"
@@ -31,13 +36,35 @@ def main : IO UInt32 := do
   IO.println s!"rv64im_accepted_artifact_trace_constructor_checks={Nightstream.Rv64IM.rv64imAcceptedArtifactTraceConstructorChecks}"
   IO.println s!"rv64im_accepted_artifact_kernel_constructor_checks={Nightstream.Rv64IM.rv64imAcceptedArtifactKernelConstructorChecks}"
   IO.println s!"rv64im_accepted_artifact_constructor_reports={reprStr Nightstream.Rv64IM.rv64imAcceptedArtifactConstructorReports}"
+  IO.println s!"rv64im_accepted_artifact_root_execution_checks={Nightstream.Rv64IM.rv64imAcceptedArtifactRootExecutionClosureChecks}"
+  IO.println s!"rv64im_accepted_artifact_root_execution_reports={reprStr Nightstream.Rv64IM.rv64imAcceptedArtifactRootExecutionClosureReports}"
+  IO.println s!"rv64im_accepted_artifact_kernel_design_bridge_checks={Nightstream.Rv64IM.rv64imAcceptedArtifactKernelDesignBridgeClosureChecks}"
+  IO.println s!"rv64im_accepted_artifact_kernel_design_bridge_reports={reprStr Nightstream.Rv64IM.rv64imAcceptedArtifactKernelDesignBridgeClosureReports}"
+  IO.println s!"rv64im_accepted_artifact_kernel_design_bridge_rust_export_blockers={reprStr Nightstream.Rv64IM.uniqueKernelDesignBridgeRustExportBlockers}"
+  IO.println s!"rv64im_accepted_artifact_root_execution_semantics_checks={Nightstream.Rv64IM.rv64imAcceptedArtifactRootExecutionSemanticsClosureChecks}"
+  IO.println s!"rv64im_accepted_artifact_root_execution_semantics_reports={reprStr Nightstream.Rv64IM.rv64imAcceptedArtifactRootExecutionSemanticsClosureReports}"
+  IO.println s!"rv64im_accepted_artifact_root_execution_semantics_rust_export_blockers={reprStr Nightstream.Rv64IM.uniqueRootExecutionSemanticsRustExportBlockers}"
+  IO.println s!"rv64im_accepted_artifact_backend_refinement_checks={Nightstream.Rv64IM.rv64imAcceptedArtifactBackendRefinementChecks}"
+  IO.println s!"rv64im_accepted_artifact_backend_refinement_reports={reprStr Nightstream.Rv64IM.rv64imAcceptedArtifactBackendRefinementReports}"
+  IO.println s!"rv64im_accepted_artifact_backend_refinement_rust_export_blockers={reprStr Nightstream.Rv64IM.uniqueBackendRefinementRustExportBlockers}"
+  IO.println s!"rv64im_proof_complete_static_checks={reprStr Nightstream.Rv64IM.proofCompleteStaticChecks}"
+  IO.println s!"rv64im_proof_complete_static_failures={reprStr Nightstream.Rv64IM.proofCompleteStaticFailures}"
+  IO.println s!"rv64im_proof_complete_case_checks={Nightstream.Rv64IM.rv64imProofCompleteChecks}"
+  IO.println s!"rv64im_proof_complete_reports={reprStr Nightstream.Rv64IM.rv64imProofCompleteReports}"
+  IO.println s!"rv64im_proof_complete_rust_export_blockers={reprStr Nightstream.Rv64IM.uniqueProofCompleteRustExportBlockers}"
+  IO.println s!"rv64im_proof_complete_closure_blockers={reprStr Nightstream.Rv64IM.uniqueProofCompleteClosureBlockers}"
+  IO.println s!"rv64im_proof_complete_closure={Nightstream.Rv64IM.validRv64imProofCompleteClosure}"
   if Nightstream.Chip8.validGeneratedChip8ProtocolCases &&
       Nightstream.Rv64IM.validGeneratedRv64imParityCases &&
       Nightstream.Rv64IM.validGeneratedRv64imAcceptedArtifactCases &&
       Nightstream.Rv64IM.validGeneratedRv64imAcceptedArtifactNegativeCases &&
       Nightstream.Rv64IM.validGeneratedRv64imAcceptedArtifactCompletenessCases &&
       Nightstream.Rv64IM.validGeneratedRv64imAcceptedArtifactTraceConstructorCases &&
-      Nightstream.Rv64IM.validGeneratedRv64imAcceptedArtifactKernelConstructorCases then
+      Nightstream.Rv64IM.validGeneratedRv64imAcceptedArtifactKernelConstructorCases &&
+      Nightstream.Rv64IM.validGeneratedRv64imAcceptedArtifactKernelDesignBridgeClosureCases &&
+      Nightstream.Rv64IM.validGeneratedRv64imAcceptedArtifactRootExecutionSemanticsClosureCases &&
+      Nightstream.Rv64IM.validGeneratedRv64imAcceptedArtifactBackendRefinementCases &&
+      Nightstream.Rv64IM.validRv64imProofCompleteClosure then
     pure 0
   else
     pure 1
